VST-introduction/verif_get_global_pointer_from_nest2.v
@@ -185,8 +185,8 @@ Definition get_freelist1_spec :=
 (************************ get innerlist global *************************)
 Definition t_struct_b := Tstruct _b noattr.
 
-Definition get_spec :=
- DECLARE _get
+Definition get_xx_spec :=
+ DECLARE _get_xx
   WITH sh: share, v : reptype' t_struct_b, gv: globals
   PRE  []
         PROP (readable_share sh)
@@ -200,7 +200,7 @@ Definition get_spec :=
 
 
 (************************************)
-Definition Gprog : funspecs := [get_freelist_input_spec; get_freelist_input_spec'; get_freelist1_spec; get_i_spec; get_spec].
+Definition Gprog : funspecs := [get_freelist_input_spec; get_freelist_input_spec'; get_freelist1_spec; get_i_spec; get_xx_spec].
 
 
 Lemma body_get_freelist_input_spec:  semax_body Vprog Gprog f_get_freelist_input get_freelist_input_spec.
@@ -216,7 +216,7 @@ start_function. repeat forward. Qed.
 Lemma body_get_freelist1: semax_body Vprog Gprog f_get_freelist1 get_freelist1_spec.
 Proof. start_function. repeat forward. Qed.
 
-Lemma body_get : semax_body Vprog Gprog f_get get_spec.
+Lemma body_get : semax_body Vprog Gprog f_get_xx get_xx_spec.
 Proof. start_function. simpl in v. unfold_repinj. repeat forward. Qed.
 
 (*
